LeanVerus/sst/exp_rep.lean
@@ -8,63 +8,57 @@ open sst typing
 
 variable (tenv : typ_env)  (dom_aux : ClosedTyp → Type)
 
-def val_vars tenv (Γ: context) dom_aux :=  (i : Nat) → (_ : i < Γ.length) → typ_interp tenv dom_aux Γ[i] ⊕ ExpError
+def val_vars tenv (Γ: context) dom_aux :=  (i : Nat) → (_ : i < Γ.length) → typ_interp tenv dom_aux Γ[i] --⊕ ExpError
+
+axiom div_zero_unspecified_value : Int → Int
+
+noncomputable def div_totalized_int (x y : Int) : Int :=
+  if y = 0 then div_zero_unspecified_value x else x / y
+
+noncomputable def div_totalized_nat (x y : Nat) : Int :=
+  if y = 0 then div_zero_unspecified_value x else x / y
 
 noncomputable
-def exp_rep Γ tenv (venv: val_vars tenv Γ dom_aux) (t : Typ) (e : Exp) (hty : Γ ⊢ e : t): typ_interp tenv dom_aux t ⊕ ExpError:=
+def exp_rep Γ tenv (venv: val_vars tenv Γ dom_aux) (t : Typ) (e : Exp) (hty : Γ ⊢ e : t): typ_interp tenv dom_aux t:=
   match e with
   | .Const c =>
     match c with
     | .Bool b =>
       cast_typ_interp (ty_constbool_inv b hty).symm (cast interp_bool.symm b)
-      |> .inl
     | .Int i =>
       cast_typ_interp (ty_constint_inv i hty).symm (cast interp_int.symm i)
-      |> .inl
     | .Char c =>
       cast_typ_interp (ty_constchar_inv c hty).symm (cast interp_char.symm c)
-      |> .inl
     | .Float32 f =>
       cast_typ_interp (ty_constfloat32_inv f hty).symm (cast interp_float32.symm f)
-      |> .inl
     | .Float64 f =>
       cast_typ_interp (ty_constfloat64_inv f hty).symm (cast interp_float64.symm f)
-      |> .inl
     | .StrSlice s =>
       cast_typ_interp (ty_strslice_inv s hty).symm (cast interp_strslice.symm s)
-      |> .inl
 
   | .Var i =>
-    match (venv i (ty_var_withinbound i hty)) with
-    | .inl v => cast_typ_interp (ty_var_inv i hty).symm v |> Sum.inl
-    | .inr e => Sum.inr e
+    cast_typ_interp (ty_var_inv i hty).symm (venv i (ty_var_withinbound i hty))
 
   | .ArrayLiteral es =>
     let A: Typ := Classical.choose (ty_array_inv es hty)
     let hA : t = .Array A := (Classical.choose_spec (ty_array_inv es hty)).1
-    -- (fun e ls =>
-    --   match e with
-    --   | none => .inr .RuntimeErr
-    --   | some e' => e' :: ls) []
-    let res :=
-      es.attach.map (fun e : { x: Exp // x ∈ es } =>
-        have helem :  WfTm Γ A e.1 := (Classical.choose_spec (ty_array_inv es hty)).2 e.1 e.2
-        have : sizeOf e.val < 1 + sizeOf es := by
-          refine Nat.lt_add_left 1 ?_;
-          refine List.sizeOf_lt_of_mem ?_;
-          exact e.property
-        exp_rep Γ tenv venv A e.1 helem)
-    let f : List (typ_interp tenv dom_aux A ⊕ ExpError) → List (typ_interp tenv dom_aux A) ⊕ ExpError := sorry
-    sorry
+    cast_typ_interp hA.symm
+      (cast (interp_array A).symm
+        (es.attach.map (fun e : { x: Exp // x ∈ es } =>
+          have helem :  WfTm Γ A e.1 := (Classical.choose_spec (ty_array_inv es hty)).2 e.1 e.2
+          have : sizeOf e.val < 1 + sizeOf es := by
+            refine Nat.lt_add_left 1 ?_;
+            refine List.sizeOf_lt_of_mem ?_;
+            exact e.property
+          exp_rep Γ tenv venv A e.1 helem)))
+
   | .Unaryr op arg =>
     match op with
     | .HasType t' =>
       let A: Typ := Classical.choose (ty_hasType_inv arg t' t hty).2
       let hA := Classical.choose_spec (ty_hasType_inv arg t' t hty).2
-      match (exp_rep Γ tenv venv A arg hA) with
-      | .inl _ =>
-        cast_typ_interp (ty_hasType_inv arg t' t hty).1.symm (cast interp_bool.symm ((typ_subst tenv A).1 = (typ_subst tenv t').1)) |> .inl
-      | .inr e => .inr e
+      cast_typ_interp (ty_hasType_inv arg t' t hty).1.symm (cast interp_bool.symm ((typ_subst tenv A).1 = (typ_subst tenv t').1))
+
     | .Box t' => sorry
     | .Unbox t' => sorry
     | .IsVariant dt var => sorry
@@ -73,18 +67,19 @@ def exp_rep Γ tenv (venv: val_vars tenv Γ dom_aux) (t : Typ) (e : Exp) (hty : 
   | .Unary op arg =>
     match op with
     | .Not =>
-      match (exp_rep Γ tenv venv t arg (ty_not_inv arg hty).2) with
-      | .inl r =>
-        let res_bool :=
-          cast_typ_interp (ty_not_inv arg hty).1 r
-          |> cast interp_bool
-        cast_typ_interp (ty_not_inv arg hty).1.symm (cast interp_bool.symm ¬res_bool)
-        |> .inl
-      | .inr e => .inr e
+      let res_bool :=
+        cast_typ_interp
+          (ty_not_inv arg hty).1
+          (exp_rep Γ tenv venv t arg (ty_not_inv arg hty).2)
+        |> cast interp_bool
+      cast_typ_interp (ty_not_inv arg hty).1.symm (cast interp_bool.symm ¬res_bool)
 
     | .FloatToBits =>
       match arg with
       | _ => sorry
+      -- match (ty_floatToBits_inv arg hty) with
+      -- | Or.inl hl => sorry
+      -- | Or.inr hr => sorry
     | .BitNot (width : Option Nat) => sorry
     | .Clip (range : IntRange) (truncate : Bool) => sorry
 
@@ -92,121 +87,139 @@ def exp_rep Γ tenv (venv: val_vars tenv Γ dom_aux) (t : Typ) (e : Exp) (hty : 
   | .Binary op arg₁ arg₂ =>
     match op with
     | .And =>
-      match (exp_rep Γ tenv venv t arg₁ (ty_and_inv arg₁ arg₂ hty).2.1), (exp_rep Γ tenv venv t arg₂ (ty_and_inv arg₁ arg₂ hty).2.2) with
-      | .inl r₁, .inl r₂ =>
-        let l_bool :=
-          cast_typ_interp (ty_and_inv arg₁ arg₂ hty).1 r₁
-          |> cast interp_bool
-        let r_bool :=
-          cast_typ_interp (ty_and_inv arg₁ arg₂ hty).1 r₂
-          |> cast interp_bool
-        cast_typ_interp (ty_and_inv arg₁ arg₂ hty).1.symm (cast interp_bool.symm (l_bool ∧ r_bool))
-        |> .inl
-      | .inl _, .inr e | .inr e, .inl _ | .inr e, .inr _ => .inr e
-
+      let l_bool :=
+        cast_typ_interp
+          (ty_and_inv arg₁ arg₂ hty).1
+          (exp_rep Γ tenv venv t arg₁ (ty_and_inv arg₁ arg₂ hty).2.1)
+        |> cast interp_bool
+      let r_bool :=
+        cast_typ_interp
+          (ty_and_inv arg₁ arg₂ hty).1
+          (exp_rep Γ tenv venv t arg₂ (ty_and_inv arg₁ arg₂ hty).2.2)
+        |> cast interp_bool
+      cast_typ_interp (ty_and_inv arg₁ arg₂ hty).1.symm (cast interp_bool.symm (l_bool ∧ r_bool))
 
     | .Or =>
-      match (exp_rep Γ tenv venv t arg₁ (ty_or_inv arg₁ arg₂ hty).2.1), (exp_rep Γ tenv venv t arg₂ (ty_or_inv arg₁ arg₂ hty).2.2) with
-      | .inl r₁, .inl r₂ =>
-        let l_bool :=
-          cast_typ_interp (ty_or_inv arg₁ arg₂ hty).1 r₁
-          |> cast interp_bool
-        let r_bool :=
-          cast_typ_interp (ty_or_inv arg₁ arg₂ hty).1 r₂
-          |> cast interp_bool
-        cast_typ_interp (ty_or_inv arg₁ arg₂ hty).1.symm (cast interp_bool.symm (l_bool ∨ r_bool))
-        |> .inl
-      | .inl _, .inr e | .inr e, .inl _ | .inr e, .inr _ => .inr e
+      let l_bool :=
+        cast_typ_interp
+          (ty_or_inv arg₁ arg₂ hty).1
+          (exp_rep Γ tenv venv t arg₁ (ty_or_inv arg₁ arg₂ hty).2.1)
+        |> cast interp_bool
+      let r_bool :=
+        cast_typ_interp
+          (ty_or_inv arg₁ arg₂ hty).1
+          (exp_rep Γ tenv venv t arg₂ (ty_or_inv arg₁ arg₂ hty).2.2)
+        |> cast interp_bool
+      cast_typ_interp (ty_or_inv arg₁ arg₂ hty).1.symm (cast interp_bool.symm (l_bool ∨ r_bool))
 
     | .Xor =>
-      match (exp_rep Γ tenv venv t arg₁ (ty_xor_inv arg₁ arg₂ hty).2.1), (exp_rep Γ tenv venv t arg₂ (ty_xor_inv arg₁ arg₂ hty).2.2) with
-      | .inl r₁, .inl r₂ =>
-        let l_bool :=
-          cast_typ_interp (ty_xor_inv arg₁ arg₂ hty).1 r₁
-          |> cast interp_bool
-        let r_bool :=
-          cast_typ_interp (ty_xor_inv arg₁ arg₂ hty).1 r₂
-          |> cast interp_bool
-        cast_typ_interp (ty_xor_inv arg₁ arg₂ hty).1.symm (cast interp_bool.symm (Xor' l_bool r_bool))
-        |> .inl
-      | .inl _, .inr e | .inr e, .inl _ | .inr e, .inr _ => .inr e
+      let l_bool :=
+        cast_typ_interp
+          (ty_xor_inv arg₁ arg₂ hty).1
+          (exp_rep Γ tenv venv t arg₁ (ty_xor_inv arg₁ arg₂ hty).2.1)
+        |> cast interp_bool
+      let r_bool :=
+        cast_typ_interp
+          (ty_xor_inv arg₁ arg₂ hty).1
+          (exp_rep Γ tenv venv t arg₂ (ty_xor_inv arg₁ arg₂ hty).2.2)
+        |> cast interp_bool
+      cast_typ_interp (ty_xor_inv arg₁ arg₂ hty).1.symm (cast interp_bool.symm (Xor' l_bool r_bool))
 
     | .Implies =>
-      match (exp_rep Γ tenv venv t arg₁ (ty_implies_inv arg₁ arg₂ hty).2.1), (exp_rep Γ tenv venv t arg₂ (ty_implies_inv arg₁ arg₂ hty).2.2) with
-      | .inl r₁, .inl r₂ =>
-        let l_bool :=
-          cast_typ_interp (ty_implies_inv arg₁ arg₂ hty).1 r₁
-          |> cast interp_bool
-        let r_bool :=
-          cast_typ_interp (ty_implies_inv arg₁ arg₂ hty).1 r₂
-          |> cast interp_bool
-        cast_typ_interp (ty_implies_inv arg₁ arg₂ hty).1.symm (cast interp_bool.symm (l_bool → r_bool))
-        |> .inl
-      | .inl _, .inr e | .inr e, .inl _ | .inr e, .inr _ => .inr e
+      let l_bool :=
+        cast_typ_interp
+          (ty_implies_inv arg₁ arg₂ hty).1
+          (exp_rep Γ tenv venv t arg₁ (ty_implies_inv arg₁ arg₂ hty).2.1)
+        |> cast interp_bool
+      let r_bool :=
+        cast_typ_interp
+          (ty_implies_inv arg₁ arg₂ hty).1
+          (exp_rep Γ tenv venv t arg₂ (ty_implies_inv arg₁ arg₂ hty).2.2)
+        |> cast interp_bool
+      cast_typ_interp (ty_implies_inv arg₁ arg₂ hty).1.symm (cast interp_bool.symm (l_bool → r_bool))
 
     | .Inequality (op : InequalityOp) =>
-      let l_res := exp_rep Γ tenv venv (Typ.Int .Int) arg₁ (ty_ineq_inv arg₁ arg₂ op hty).2.1
-      let r_res := exp_rep Γ tenv venv (Typ.Int .Int) arg₂ (ty_ineq_inv arg₁ arg₂ op hty).2.2
-      match l_res, r_res with
-      | .inl r₁, .inl r₂ =>
-        let l_int := cast interp_int r₁
-        let r_int := cast interp_int r₂
-        let res :=
-          match op with
-          | .Le => l_int <= r_int
-          | .Ge => l_int >= r_int
-          | .Lt => l_int < r_int
-          | .Gt => l_int > r_int
-        cast_typ_interp (ty_ineq_inv arg₁ arg₂ op hty).1.symm (cast interp_bool.symm res) |> .inl
-      | .inl _, .inr e | .inr e, .inl _ | .inr e, .inr _ => .inr e
+      let l_int :=
+        exp_rep Γ tenv venv (Typ.Int .Int) arg₁ (ty_ineq_inv arg₁ arg₂ op hty).2.1
+        |> cast interp_int
+      let r_int :=
+        exp_rep Γ tenv venv (Typ.Int .Int) arg₂ (ty_ineq_inv arg₁ arg₂ op hty).2.2
+        |> cast interp_int
+      let res :=
+        match op with
+        | .Le => l_int <= r_int
+        | .Ge => l_int >= r_int
+        | .Lt => l_int < r_int
+        | .Gt => l_int > r_int
+      cast_typ_interp (ty_ineq_inv arg₁ arg₂ op hty).1.symm (cast interp_bool.symm res)
 
     | .Ne =>
       let A: Typ := Classical.choose (ty_ne_inv arg₁ arg₂ hty).2
       let hty₁ : Γ ⊢ arg₁ : A := (Classical.choose_spec (ty_ne_inv arg₁ arg₂ hty).2).1
       let hty₂ : Γ ⊢ arg₂ : A := (Classical.choose_spec (ty_ne_inv arg₁ arg₂ hty).2).2
-      match (exp_rep Γ tenv venv A arg₁ hty₁), (exp_rep Γ tenv venv A arg₂ hty₂) with
-      | .inl r₁, .inl r₂ => sorry
-        --cast_typ_interp (ty_ne_inv arg₁ arg₂ hty).1.symm (cast interp_bool.symm (r₁ ≠ r₂)) |> .inl
-      | .inl _, .inr e | .inr e, .inl _ | .inr e, .inr _ => .inr e
+      let rep₁ := exp_rep Γ tenv venv A arg₁ hty₁
+      let rep₂ := exp_rep Γ tenv venv A arg₂ hty₂
+      cast_typ_interp (ty_ne_inv arg₁ arg₂ hty).1.symm (cast interp_bool.symm (@Decidable.decide (rep₁ = rep₂) (Classical.propDecidable (rep₁ = rep₂))))
 
     | .Eq m =>
       let A: Typ := Classical.choose (ty_eq_inv arg₁ arg₂ m hty).2
       let hty₁ : Γ ⊢ arg₁ : A := (Classical.choose_spec (ty_eq_inv arg₁ arg₂ m hty).2).1
       let hty₂ : Γ ⊢ arg₂ : A := (Classical.choose_spec (ty_eq_inv arg₁ arg₂ m hty).2).2
-      match (exp_rep Γ tenv venv A arg₁ hty₁), (exp_rep Γ tenv venv A arg₂ hty₂) with
-      | .inl r₁, .inl r₂ => sorry
-        -- cast_typ_interp (ty_eq_inv arg₁ arg₂ m hty).1.symm (cast interp_bool.symm (r₁ = r₂)) |> .inl
-      | .inl _, .inr e | .inr e, .inl _ | .inr e, .inr _ => .inr e
+      let rep₁ := exp_rep Γ tenv venv A arg₁ hty₁
+      let rep₂ := exp_rep Γ tenv venv A arg₂ hty₂
+      cast_typ_interp (ty_eq_inv arg₁ arg₂ m hty).1.symm (cast interp_bool.symm (@Decidable.decide (rep₁ = rep₂) (Classical.propDecidable (rep₁ = rep₂))))
 
-    -- bound checking?
+    -- TODO: look at ARRAY_INDEX in ast examples.
     | .Index (ak : ArrayKind) =>
       match ak with
-      | .Slice => sorry
       | .Array => sorry
+      | .Slice => sorry
+
 
     | .Arith op =>
       match op with
       | .Add =>
         match t with
         | .Int .Int =>
-          let l_res := exp_rep Γ tenv venv (Typ.Int .Int) arg₁ (ty_add_inv arg₁ arg₂ (.Int .Int) hty).2.1
-          let r_res := exp_rep Γ tenv venv (Typ.Int .Int) arg₂ (ty_add_inv arg₁ arg₂ (.Int .Int) hty).2.2
-          match l_res, r_res with
-          | .inl r₁, .inl r₂ =>
-            let l_int := cast interp_int r₁
-            let r_int := cast interp_int r₂
-            cast interp_int.symm (l_int + r_int) |> .inl
-          | .inl _, .inr e | .inr e, .inl _ | .inr e, .inr _ => .inr e
+          let l_int :=
+            exp_rep Γ tenv venv (Typ.Int .Int) arg₁ (ty_add_inv arg₁ arg₂ (.Int .Int) hty).2.1
+            |> cast interp_int
+          let r_int :=
+            exp_rep Γ tenv venv (Typ.Int .Int) arg₂ (ty_add_inv arg₁ arg₂ (.Int .Int) hty).2.2
+            |> cast interp_int
+          cast interp_int.symm (l_int + r_int)
         | .Int .Nat =>
-          let l_res := exp_rep Γ tenv venv (Typ.Int .Nat) arg₁ (ty_add_inv arg₁ arg₂ (.Int .Nat) hty).2.1
-          let r_res := exp_rep Γ tenv venv (Typ.Int .Nat) arg₂ (ty_add_inv arg₁ arg₂ (.Int .Nat) hty).2.2
-          match l_res, r_res with
-          | .inl r₁, .inl r₂ =>
-            let l_nat := cast interp_nat r₁
-            let r_nat := cast interp_nat r₂
-            cast interp_nat.symm (l_nat + r_nat) |> .inl
-          | .inl _, .inr e | .inr e, .inl _ | .inr e, .inr _ => .inr e
+          let l_nat :=
+            exp_rep Γ tenv venv (Typ.Int .Nat) arg₁ (ty_add_inv arg₁ arg₂ (.Int .Nat) hty).2.1
+            |> cast interp_nat
+          let r_nat :=
+            exp_rep Γ tenv venv (Typ.Int .Nat) arg₂ (ty_add_inv arg₁ arg₂ (.Int .Nat) hty).2.2
+            |> cast interp_nat
+          cast interp_nat.symm (l_nat + r_nat)
+
+        -- TODO: How to say this is impossible?
         | _ => sorry
+
+      | .EuclideanDiv =>
+        let t_arg :=
+        match (ty_div_inv arg₁ arg₂ t hty).2 with
+        | Or.inl ⟨h₁, _⟩ => extract_typ h₁
+          -- let l_int :=
+          --   exp_rep Γ tenv venv (Typ.Int .Int) arg₁ h₁
+          --   |> cast interp_int
+          -- let r_int :=
+          --   exp_rep Γ tenv venv (Typ.Int .Int) arg₂ h₂
+          --   |> cast interp_int
+          -- cast_typ_interp (ty_div_inv arg₁ arg₂ t hty).1.symm (cast interp_int.symm (div_totalized_int l_int r_int))
+        | Or.inr ⟨h₁, _⟩ => extract_typ h₁
+          -- let l_nat :=
+          --   exp_rep Γ tenv venv (Typ.Int .Nat) arg₁ h₁
+          --   |> cast interp_nat
+          -- let r_nat :=
+          --   exp_rep Γ tenv venv (Typ.Int .Nat) arg₂ h₂
+          --   |> cast interp_nat
+          -- cast_typ_interp (ty_div_inv arg₁ arg₂ t hty).1.symm (cast interp_int.symm (div_totalized_int l_nat r_nat))
+        sorry
       | _ => sorry
     | .Bitwise (op : BitwiseOp) (mode : Mode) => sorry
 
@@ -214,11 +227,9 @@ def exp_rep Γ tenv (venv: val_vars tenv Γ dom_aux) (t : Typ) (e : Exp) (hty : 
     let c_res := exp_rep Γ tenv venv Typ._Bool c (ty_if_inv c b₁ b₂ t hty).1
     let b₁_res := exp_rep Γ tenv venv t b₁ (ty_if_inv c b₁ b₂ t hty).2.1
     let b₂_res := exp_rep Γ tenv venv t b₂ (ty_if_inv c b₁ b₂ t hty).2.2
-    match c_res, b₁_res, b₂_res with
-    | .inl c', .inl b₁', .inl b₂' =>
-      let c_bool := cast interp_bool c'
-      (if c_bool then b₁' else b₂') |> .inl
-    | .inr e, _, _ | _, .inr e, _ | _, _, .inr e => .inr e
+    let c_bool := cast interp_bool c_res
+    if c_bool then b₁_res else b₂_res
+
   | .Let (tys : List Typ) (es : List Exp) (body : Exp) => sorry
   | .Quant (q : Quant) (var : Typ) (body : Exp) => sorry
   | .TupleCtor (size : Nat) (data : List Exp) => sorry
@@ -229,4 +240,222 @@ def exp_rep Γ tenv (venv: val_vars tenv Γ dom_aux) (t : Typ) (e : Exp) (hty : 
   | .StructCtor (dt : Ident) (fields : List (String × Exp)) => sorry
   | .Lambda (var : Typ) (exp : Exp) => sorry
 
-termination_by sizeOf e
+-- noncomputable
+-- def exp_rep Γ tenv (venv: val_vars tenv Γ dom_aux) (t : Typ) (e : Exp) (hty : Γ ⊢ e : t): typ_interp tenv dom_aux t ⊕ ExpError:=
+--   match e with
+--   | .Const c =>
+--     match c with
+--     | .Bool b =>
+--       cast_typ_interp (ty_constbool_inv b hty).symm (cast interp_bool.symm b)
+--       |> .inl
+--     | .Int i =>
+--       cast_typ_interp (ty_constint_inv i hty).symm (cast interp_int.symm i)
+--       |> .inl
+--     | .Char c =>
+--       cast_typ_interp (ty_constchar_inv c hty).symm (cast interp_char.symm c)
+--       |> .inl
+--     | .Float32 f =>
+--       cast_typ_interp (ty_constfloat32_inv f hty).symm (cast interp_float32.symm f)
+--       |> .inl
+--     | .Float64 f =>
+--       cast_typ_interp (ty_constfloat64_inv f hty).symm (cast interp_float64.symm f)
+--       |> .inl
+--     | .StrSlice s =>
+--       cast_typ_interp (ty_strslice_inv s hty).symm (cast interp_strslice.symm s)
+--       |> .inl
+
+--   | .Var i =>
+--     match (venv i (ty_var_withinbound i hty)) with
+--     | .inl v => cast_typ_interp (ty_var_inv i hty).symm v |> Sum.inl
+--     | .inr e => Sum.inr e
+
+--   | .ArrayLiteral es =>
+--     let A: Typ := Classical.choose (ty_array_inv es hty)
+--     let hA : t = .Array A := (Classical.choose_spec (ty_array_inv es hty)).1
+--     -- (fun e ls =>
+--     --   match e with
+--     --   | none => .inr .RuntimeErr
+--     --   | some e' => e' :: ls) []
+--     let res :=
+--       es.attach.map (fun e : { x: Exp // x ∈ es } =>
+--         have helem :  WfTm Γ A e.1 := (Classical.choose_spec (ty_array_inv es hty)).2 e.1 e.2
+--         have : sizeOf e.val < 1 + sizeOf es := by
+--           refine Nat.lt_add_left 1 ?_;
+--           refine List.sizeOf_lt_of_mem ?_;
+--           exact e.property
+--         exp_rep Γ tenv venv A e.1 helem)
+--     let f : List (typ_interp tenv dom_aux A ⊕ ExpError) → List (typ_interp tenv dom_aux A) ⊕ ExpError := sorry
+--     sorry
+--   | .Unaryr op arg =>
+--     match op with
+--     | .HasType t' =>
+--       let A: Typ := Classical.choose (ty_hasType_inv arg t' t hty).2
+--       let hA := Classical.choose_spec (ty_hasType_inv arg t' t hty).2
+--       match (exp_rep Γ tenv venv A arg hA) with
+--       | .inl _ =>
+--         cast_typ_interp (ty_hasType_inv arg t' t hty).1.symm (cast interp_bool.symm ((typ_subst tenv A).1 = (typ_subst tenv t').1)) |> .inl
+--       | .inr e => .inr e
+--     | .Box t' => sorry
+--     | .Unbox t' => sorry
+--     | .IsVariant dt var => sorry
+--     | .Proj field => sorry
+
+--   | .Unary op arg =>
+--     match op with
+--     | .Not =>
+--       match (exp_rep Γ tenv venv t arg (ty_not_inv arg hty).2) with
+--       | .inl r =>
+--         let res_bool :=
+--           cast_typ_interp (ty_not_inv arg hty).1 r
+--           |> cast interp_bool
+--         cast_typ_interp (ty_not_inv arg hty).1.symm (cast interp_bool.symm ¬res_bool)
+--         |> .inl
+--       | .inr e => .inr e
+
+--     | .FloatToBits =>
+--       match arg with
+--       | _ => sorry
+--     | .BitNot (width : Option Nat) => sorry
+--     | .Clip (range : IntRange) (truncate : Bool) => sorry
+
+
+--   | .Binary op arg₁ arg₂ =>
+--     match op with
+--     | .And =>
+--       match (exp_rep Γ tenv venv t arg₁ (ty_and_inv arg₁ arg₂ hty).2.1), (exp_rep Γ tenv venv t arg₂ (ty_and_inv arg₁ arg₂ hty).2.2) with
+--       | .inl r₁, .inl r₂ =>
+--         let l_bool :=
+--           cast_typ_interp (ty_and_inv arg₁ arg₂ hty).1 r₁
+--           |> cast interp_bool
+--         let r_bool :=
+--           cast_typ_interp (ty_and_inv arg₁ arg₂ hty).1 r₂
+--           |> cast interp_bool
+--         cast_typ_interp (ty_and_inv arg₁ arg₂ hty).1.symm (cast interp_bool.symm (l_bool ∧ r_bool))
+--         |> .inl
+--       | .inl _, .inr e | .inr e, .inl _ | .inr e, .inr _ => .inr e
+
+
+--     | .Or =>
+--       match (exp_rep Γ tenv venv t arg₁ (ty_or_inv arg₁ arg₂ hty).2.1), (exp_rep Γ tenv venv t arg₂ (ty_or_inv arg₁ arg₂ hty).2.2) with
+--       | .inl r₁, .inl r₂ =>
+--         let l_bool :=
+--           cast_typ_interp (ty_or_inv arg₁ arg₂ hty).1 r₁
+--           |> cast interp_bool
+--         let r_bool :=
+--           cast_typ_interp (ty_or_inv arg₁ arg₂ hty).1 r₂
+--           |> cast interp_bool
+--         cast_typ_interp (ty_or_inv arg₁ arg₂ hty).1.symm (cast interp_bool.symm (l_bool ∨ r_bool))
+--         |> .inl
+--       | .inl _, .inr e | .inr e, .inl _ | .inr e, .inr _ => .inr e
+
+--     | .Xor =>
+--       match (exp_rep Γ tenv venv t arg₁ (ty_xor_inv arg₁ arg₂ hty).2.1), (exp_rep Γ tenv venv t arg₂ (ty_xor_inv arg₁ arg₂ hty).2.2) with
+--       | .inl r₁, .inl r₂ =>
+--         let l_bool :=
+--           cast_typ_interp (ty_xor_inv arg₁ arg₂ hty).1 r₁
+--           |> cast interp_bool
+--         let r_bool :=
+--           cast_typ_interp (ty_xor_inv arg₁ arg₂ hty).1 r₂
+--           |> cast interp_bool
+--         cast_typ_interp (ty_xor_inv arg₁ arg₂ hty).1.symm (cast interp_bool.symm (Xor' l_bool r_bool))
+--         |> .inl
+--       | .inl _, .inr e | .inr e, .inl _ | .inr e, .inr _ => .inr e
+
+--     | .Implies =>
+--       match (exp_rep Γ tenv venv t arg₁ (ty_implies_inv arg₁ arg₂ hty).2.1), (exp_rep Γ tenv venv t arg₂ (ty_implies_inv arg₁ arg₂ hty).2.2) with
+--       | .inl r₁, .inl r₂ =>
+--         let l_bool :=
+--           cast_typ_interp (ty_implies_inv arg₁ arg₂ hty).1 r₁
+--           |> cast interp_bool
+--         let r_bool :=
+--           cast_typ_interp (ty_implies_inv arg₁ arg₂ hty).1 r₂
+--           |> cast interp_bool
+--         cast_typ_interp (ty_implies_inv arg₁ arg₂ hty).1.symm (cast interp_bool.symm (l_bool → r_bool))
+--         |> .inl
+--       | .inl _, .inr e | .inr e, .inl _ | .inr e, .inr _ => .inr e
+
+--     | .Inequality (op : InequalityOp) =>
+--       let l_res := exp_rep Γ tenv venv (Typ.Int .Int) arg₁ (ty_ineq_inv arg₁ arg₂ op hty).2.1
+--       let r_res := exp_rep Γ tenv venv (Typ.Int .Int) arg₂ (ty_ineq_inv arg₁ arg₂ op hty).2.2
+--       match l_res, r_res with
+--       | .inl r₁, .inl r₂ =>
+--         let l_int := cast interp_int r₁
+--         let r_int := cast interp_int r₂
+--         let res :=
+--           match op with
+--           | .Le => l_int <= r_int
+--           | .Ge => l_int >= r_int
+--           | .Lt => l_int < r_int
+--           | .Gt => l_int > r_int
+--         cast_typ_interp (ty_ineq_inv arg₁ arg₂ op hty).1.symm (cast interp_bool.symm res) |> .inl
+--       | .inl _, .inr e | .inr e, .inl _ | .inr e, .inr _ => .inr e
+
+--     | .Ne =>
+--       let A: Typ := Classical.choose (ty_ne_inv arg₁ arg₂ hty).2
+--       let hty₁ : Γ ⊢ arg₁ : A := (Classical.choose_spec (ty_ne_inv arg₁ arg₂ hty).2).1
+--       let hty₂ : Γ ⊢ arg₂ : A := (Classical.choose_spec (ty_ne_inv arg₁ arg₂ hty).2).2
+--       match (exp_rep Γ tenv venv A arg₁ hty₁), (exp_rep Γ tenv venv A arg₂ hty₂) with
+--       | .inl r₁, .inl r₂ => sorry
+--         --cast_typ_interp (ty_ne_inv arg₁ arg₂ hty).1.symm (cast interp_bool.symm (r₁ ≠ r₂)) |> .inl
+--       | .inl _, .inr e | .inr e, .inl _ | .inr e, .inr _ => .inr e
+
+--     | .Eq m =>
+--       let A: Typ := Classical.choose (ty_eq_inv arg₁ arg₂ m hty).2
+--       let hty₁ : Γ ⊢ arg₁ : A := (Classical.choose_spec (ty_eq_inv arg₁ arg₂ m hty).2).1
+--       let hty₂ : Γ ⊢ arg₂ : A := (Classical.choose_spec (ty_eq_inv arg₁ arg₂ m hty).2).2
+--       match (exp_rep Γ tenv venv A arg₁ hty₁), (exp_rep Γ tenv venv A arg₂ hty₂) with
+--       | .inl r₁, .inl r₂ => sorry
+--         -- cast_typ_interp (ty_eq_inv arg₁ arg₂ m hty).1.symm (cast interp_bool.symm (r₁ = r₂)) |> .inl
+--       | .inl _, .inr e | .inr e, .inl _ | .inr e, .inr _ => .inr e
+
+--     | .Index (ak : ArrayKind) =>
+--       match ak with
+--       | .Slice => sorry
+--       | .Array => sorry
+
+--     | .Arith op =>
+--       match op with
+--       | .Add =>
+--         match t with
+--         | .Int .Int =>
+--           let l_res := exp_rep Γ tenv venv (Typ.Int .Int) arg₁ (ty_add_inv arg₁ arg₂ (.Int .Int) hty).2.1
+--           let r_res := exp_rep Γ tenv venv (Typ.Int .Int) arg₂ (ty_add_inv arg₁ arg₂ (.Int .Int) hty).2.2
+--           match l_res, r_res with
+--           | .inl r₁, .inl r₂ =>
+--             let l_int := cast interp_int r₁
+--             let r_int := cast interp_int r₂
+--             cast interp_int.symm (l_int + r_int) |> .inl
+--           | .inl _, .inr e | .inr e, .inl _ | .inr e, .inr _ => .inr e
+--         | .Int .Nat =>
+--           let l_res := exp_rep Γ tenv venv (Typ.Int .Nat) arg₁ (ty_add_inv arg₁ arg₂ (.Int .Nat) hty).2.1
+--           let r_res := exp_rep Γ tenv venv (Typ.Int .Nat) arg₂ (ty_add_inv arg₁ arg₂ (.Int .Nat) hty).2.2
+--           match l_res, r_res with
+--           | .inl r₁, .inl r₂ =>
+--             let l_nat := cast interp_nat r₁
+--             let r_nat := cast interp_nat r₂
+--             cast interp_nat.symm (l_nat + r_nat) |> .inl
+--           | .inl _, .inr e | .inr e, .inl _ | .inr e, .inr _ => .inr e
+--         | _ => sorry
+--       | _ => sorry
+--     | .Bitwise (op : BitwiseOp) (mode : Mode) => sorry
+
+--   | .If c b₁ b₂ =>
+--     let c_res := exp_rep Γ tenv venv Typ._Bool c (ty_if_inv c b₁ b₂ t hty).1
+--     let b₁_res := exp_rep Γ tenv venv t b₁ (ty_if_inv c b₁ b₂ t hty).2.1
+--     let b₂_res := exp_rep Γ tenv venv t b₂ (ty_if_inv c b₁ b₂ t hty).2.2
+--     match c_res, b₁_res, b₂_res with
+--     | .inl c', .inl b₁', .inl b₂' =>
+--       let c_bool := cast interp_bool c'
+--       (if c_bool then b₁' else b₂') |> .inl
+--     | .inr e, _, _ | _, .inr e, _ | _, _, .inr e => .inr e
+--   | .Let (tys : List Typ) (es : List Exp) (body : Exp) => sorry
+--   | .Quant (q : Quant) (var : Typ) (body : Exp) => sorry
+--   | .TupleCtor (size : Nat) (data : List Exp) => sorry
+
+
+--   | .Call (fn : CallFun) (typs : List Typ) (exps : List Exp) (ret : Typ) => sorry
+--   | .CallLambda (lam : Exp) (arg : Exp) => sorry
+--   | .StructCtor (dt : Ident) (fields : List (String × Exp)) => sorry
+--   | .Lambda (var : Typ) (exp : Exp) => sorry
+
+-- termination_by sizeOf e
